importing deduction proof, changing term substitution notation

theories/FOL/Reductions/PCPb_to_ZFD.v
@@ -5,7 +5,6 @@ Require Import Undecidability.FOL.Util.FullTarski.
 Require Import Undecidability.FOL.Util.FullDeduction.
 Require Import Undecidability.FOL.ZF.
 Require Import Undecidability.FOL.Reductions.PCPb_to_ZF.
-Require Import Lia.
 
 From Undecidability.PCP Require Import PCP Util.PCP_facts Reductions.PCPb_iff_dPCPb.
 
@@ -15,10 +14,675 @@ Import ListAutomationNotations.
 Local Set Implicit Arguments.
 Local Unset Strict Implicit.
 
+
+
+
+(** ** Simple derivations in ZF *)
+
+Close Scope sem.
+
+Lemma ZF_eset x :
+  ZFeq' ⊢I ¬ (x ∈ ∅).
+Proof.
+  change (ZFeq' ⊢I (¬ ($0 ∈ ∅))[x..]).
+  apply AllE. apply Ctx. firstorder.
+Qed.
+
+Lemma ZF_eset' T x :
+  ZFeq' <<= T -> T ⊢I ¬ (x ∈ ∅).
+Proof.
+  intros H. now apply (Weak (ZF_eset x)).
+Qed.
+
+Fixpoint tnumeral n :=
+  match n with 
+  | O => ∅
+  | S n => σ (tnumeral n)
+end.
+
+Lemma ZF_numeral n :
+  ZFeq' ⊢I tnumeral n ∈ ω.
+Proof.
+  induction n; cbn.
+  - eapply CE1. apply Ctx. firstorder.
+  - eapply IE; try apply IHn.
+    change (ZFeq' ⊢I ($0 ∈ ω --> σ ($0) ∈ ω)[(tnumeral n)..]).
+    apply AllE. eapply CE2. apply Ctx. firstorder.
+Qed.
+
+Lemma ZF_refl' T x :
+  ZFeq' <<= T -> T ⊢I x ≡ x.
+Proof.
+  intros H. change (T ⊢I ($0 ≡ $0)[x..]).
+  apply AllE. apply Ctx. firstorder.
+Qed.
+
+Lemma ZF_refl x :
+  ZFeq' ⊢I x ≡ x.
+Proof.
+  now apply ZF_refl'.
+Qed.
+
+Lemma ZF_sym' T x y :
+  ZFeq' <<= T -> T ⊢I x ≡ y -> T ⊢I y ≡ x.
+Proof.
+  intros H1 H2. eapply IE; try apply H2.
+  assert (H : T ⊢I ax_sym) by (apply Ctx; firstorder).
+  apply (AllE x), (AllE y) in H; cbn in H.
+
+  rewrite (subst_term_comp x (S >> var) (y..)) in H.
+Qed.
+
+Lemma ZF_trans' T x y z :
+  ZFeq' <<= T -> T ⊢I x ≡ y -> T ⊢I y ≡ z -> T ⊢I x ≡ z.
+Proof.
+  intros H1 H2 H3. eapply IE; try apply H3.
+  eapply IE; try apply H2.
+  assert (H : T ⊢I ax_trans) by (apply Ctx; firstorder).
+  now apply (AllE x), (AllE y), (AllE z) in H; cbn in H; asimpl in H.
+Qed.
+
+Lemma ZF_eq_elem T x y x' y' :
+  ZFeq' <<= T -> T ⊢I x ≡ x' -> T ⊢I y ≡ y' -> T ⊢I x ∈ y -> T ⊢I x' ∈ y'.
+Proof.
+  intros H1 H2 H3 H4. eapply IE; try apply H4.
+  eapply IE; try apply H3. eapply IE; try apply H2.
+  assert (H : T ⊢I ax_eq_elem) by (apply Ctx; firstorder).
+  now apply (AllE x), (AllE y), (AllE x'), (AllE y') in H; cbn in H; asimpl in H.
+Qed.
+
+Lemma ZF_ext' T x y :
+  ZFeq' <<= T -> T ⊢I sub x y -> T ⊢I sub y x -> T ⊢I x ≡ y.
+Proof.
+  intros H1 H2 H3. eapply IE; try apply H3.
+  eapply IE; try apply H2.
+  assert (H : T ⊢I ax_ext) by (apply Ctx; firstorder).
+  now apply (AllE x), (AllE y) in H; cbn in H; asimpl in H.
+Qed.
+
+Lemma ZF_pair_el' (T : theory) x y z :
+  ZFeq' <<= T -> T ⊢I (z ≡ x ∨ z ≡ y) <-> T ⊢I z ∈ {x; y}.
+Proof.
+  intros HT; split; intros H; eapply IE; try apply H.
+  all: assert (HP : T ⊢I ax_pair) by (apply Ctx; firstorder).
+  all: apply (AllE y), (AllE x), (AllE z) in HP; cbn in HP; asimpl in HP.
+  - eapply CE2, HP.
+  - eapply CE1, HP.
+Qed.
+
+Lemma ZF_pair_el x y z :
+  ZFeq' ⊢I (z ≡ x ∨ z ≡ y) -> ZFeq' ⊢I z ∈ {x; y}.
+Proof.
+  now apply ZF_pair_el'.
+Qed.
+
+Lemma ZF_sub_pair' x y x' y' :
+  ZFeq' ⊢I x ≡ x' --> y ≡ y'--> sub ({x; y}) ({x'; y'}).
+Proof.
+  repeat apply impl. apply bt_all. intros z. cbn. asimpl.
+  apply impl. apply ZF_pair_el'. repeat solve_tsub. eapply DE.
+  - eapply ZF_pair_el'. repeat solve_tsub. apply prv_T1.
+  - apply DI1. eapply ZF_trans'. repeat solve_tsub.
+    apply prv_T1. apply Ctx. unfold extend, contains. tauto.
+  - apply DI2. eapply ZF_trans'. repeat solve_tsub.
+    apply prv_T1. apply Ctx. unfold extend, contains. tauto.
+Qed.
+
+Lemma ZF_eq_pair' x y x' y' :
+  ZFeq' ⊢I x ≡ x' --> y ≡ y'--> {x; y} ≡ {x'; y'}.
+Proof.
+  repeat apply impl. apply ZF_ext'; trivial. solve_tsub.
+  all: eapply IE. 1,3: eapply IE. 1,3: eapply Weak_T.
+  1,3: apply ZF_sub_pair'. 1,2: solve_tsub.
+  apply prv_T2. apply ZF_sym'; try apply prv_T2. solve_tsub.
+  apply prv_T1. apply ZF_sym'; try apply prv_T1. solve_tsub.
+Qed.
+
+Lemma ZF_eq_pair T x y x' y' :
+  ZFeq' <<= T -> T ⊢I x ≡ x' -> T ⊢I y ≡ y' -> T ⊢I {x; y} ≡ {x'; y'}.
+Proof.
+  intros HT H1 H2. eapply IE; try apply H2.
+  eapply IE; try apply H1. eapply Weak_T; eauto.
+  apply ZF_eq_pair'.
+Qed.
+
+Lemma ZF_eq_opair T x y x' y' :
+  ZFeq' <<= T -> T ⊢I x ≡ x' -> T ⊢I y ≡ y' -> T ⊢I opair x y ≡ opair x' y'.
+Proof.
+  intros HT H1 H2. repeat apply ZF_eq_pair; trivial.
+Qed.
+
+Lemma ZF_sing_el x :
+  ZFeq' ⊢I x ∈ (sing x).
+Proof.
+  apply ZF_pair_el. apply DI1. apply ZF_refl.
+Qed.
+
+Lemma ZF_sing_iff T x y :
+  ZFeq' <<= T -> T ⊢I x ∈ sing y <-> T ⊢I x ≡ y.
+Proof.
+  intros HT. unfold sing.
+  rewrite <- ZF_pair_el'; trivial.
+  split; intros H.
+  - now apply DS.
+  - now apply DI1.
+Qed.
+
+Lemma ZF_union_el' (T : theory) x y z :
+  ZFeq' <<= T -> T ⊢I y ∈ x ∧ z ∈ y -> T ⊢I z ∈ ⋃ x.
+Proof.
+  intros HT H.
+  assert (HU : T ⊢I ax_union) by (apply Ctx; firstorder).
+  apply (AllE x), (AllE z) in HU; cbn in HU; asimpl in HU.
+  apply CE2 in HU. eapply IE; try apply HU.
+  apply ExI with y. cbn. asimpl. apply H.
+Qed.
+
+Lemma ZF_union_el x y z :
+  ZFeq' ⊢I y ∈ x ∧ z ∈ y -> ZFeq' ⊢I z ∈ ⋃ x.
+Proof.
+  now apply ZF_union_el'.
+Qed.
+
+Lemma ZF_sub_union {T} {HB : bounded_theory T} x y :
+  ZFeq' <<= T -> T ⊢I x ≡ y -> T ⊢I sub (⋃ x) (⋃ y).
+Proof.
+  intros HT H. apply bt_all. intros z. cbn. asimpl. 
+  apply impl. assert1 H'.
+  assert (HU : T ⋄ (z ∈ ⋃ x) ⊢I ax_union) by (apply Ctx; firstorder).
+  apply (AllE x), (AllE z) in HU; cbn in HU; asimpl in HU.
+  apply CE1 in HU. eapply (mp HU) in H'.
+  use_exists H' u. cbn. asimpl. clear H' HU.
+  eapply ZF_union_el'. repeat solve_tsub. apply CI.
+  - eapply ZF_eq_elem. repeat solve_tsub. apply ZF_refl'. repeat solve_tsub.
+    apply (Weak_T H). repeat solve_tsub. eapply CE1, prv_T1.
+  - eapply CE2, prv_T1.
+Qed.
+
+Lemma ZF_eq_union {T} {HB : bounded_theory T} x y :
+  ZFeq' <<= T -> T ⊢I x ≡ y -> T ⊢I ⋃ x ≡ ⋃ y.
+Proof.
+  intros HT H. apply ZF_ext'; try apply ZF_sub_union; trivial.
+  now apply ZF_sym'.
+Qed.
+
+Lemma ZF_bunion_el' T x y z :
+  ZFeq' <<= T -> T ⊢I (z ∈ x ∨ z ∈ y) -> T ⊢I z ∈ x ∪ y.
+Proof.
+  intros HT H. apply (DE H).
+  - eapply ZF_union_el' with x. solve_tsub. apply CI; try apply prv_T1.
+    apply ZF_pair_el'. solve_tsub. apply DI1. apply ZF_refl'. solve_tsub.
+  - eapply ZF_union_el' with y. solve_tsub. apply CI; try apply prv_T1.
+    apply ZF_pair_el'. solve_tsub. apply DI2. apply ZF_refl'. solve_tsub.
+Qed.
+
+Lemma ZF_bunion_el x y z :
+  ZFeq' ⊢I (z ∈ x ∨ z ∈ y) -> ZFeq' ⊢I z ∈ x ∪ y.
+Proof.
+  now apply ZF_bunion_el'.
+Qed.
+
+Lemma ZF_bunion_inv' x y z :
+   ZFeq' ⊢I z ∈ x ∪ y --> z ∈ x ∨ z ∈ y.
+Proof.
+  assert (TU : ZFeq' ⊢I ax_union) by (apply Ctx; firstorder).
+  pose (upair (x y : term) := {x; y}).
+  eapply (AllE (upair x y)), (AllE z) in TU; fold subst_form in TU.
+  apply CE1 in TU; fold subst_form in TU. cbn in TU; asimpl in TU.
+  apply (imps TU). apply impl.
+  assert1 H. use_exists H u. cbn. asimpl. clear H. apply prv_clear2.
+  eapply DE. apply ZF_pair_el'. repeat solve_tsub.
+  + eapply CE1. apply prv_T1.
+  + apply DI1. eapply ZF_eq_elem. repeat solve_tsub.
+    apply ZF_refl'. repeat solve_tsub. apply prv_T1.
+    eapply CE2. apply prv_T2.
+  + apply DI2. eapply ZF_eq_elem. repeat solve_tsub.
+    apply ZF_refl'. repeat solve_tsub. apply prv_T1.
+    eapply CE2. apply prv_T2.
+Qed.
+
+Lemma ZF_bunion_inv T x y z :
+   ZFeq' <<= T -> T ⊢I z ∈ x ∪ y -> T ⊢I z ∈ x ∨ z ∈ y.
+Proof.
+  intros HT H. eapply IE; try apply H.
+  eapply Weak_T; try apply HT. apply ZF_bunion_inv'.
+Qed.
+
+Lemma ZF_eq_bunion {T} {HB : bounded_theory T} x y x' y' :
+  ZFeq' <<= T -> T ⊢I x ≡ x' -> T ⊢I y ≡ y' -> T ⊢I x ∪ y ≡ x' ∪ y'.
+Proof.
+  intros HT H1 H2. now apply ZF_eq_union, ZF_eq_pair.
+Qed.
+
+Lemma ZF_sig_el T x :
+   ZFeq' <<= T -> T ⊢I x ∈ σ x.
+Proof.
+  intros H. apply ZF_bunion_el'; trivial.
+  apply DI2. apply ZF_sing_iff; trivial.
+  apply ZF_refl'. trivial.
+Qed.
+
+Lemma ZF_eq_sig {T} {HB : bounded_theory T} x y :
+  ZFeq' <<= T -> T ⊢I x ≡ y -> T ⊢I σ x ≡ σ y.
+Proof.
+  intros HT H. now apply ZF_eq_bunion, ZF_eq_pair.
+Qed.
+
+Lemma sing_pair1 T x y z :
+  ZFeq' <<= T -> T ⊢I sing x ≡ {y; z} -> T ⊢I x ≡ y.
+Proof.
+  intros HT H. apply ZF_sym'; trivial.
+  apply ZF_sing_iff; trivial. eapply ZF_eq_elem; trivial.
+  apply ZF_refl'; trivial. apply ZF_sym'; eauto.
+  apply ZF_pair_el'; trivial. apply DI1. now apply ZF_refl'.
+Qed.
+
+Lemma sing_pair2 T x y z :
+  ZFeq' <<= T -> T ⊢I sing x ≡ {y; z} -> T ⊢I x ≡ z.
+Proof.
+  intros HT H. apply ZF_sym'; trivial.
+  apply ZF_sing_iff; trivial. eapply ZF_eq_elem; trivial.
+  apply ZF_refl'; trivial. apply ZF_sym'; eauto.
+  apply ZF_pair_el'; trivial. apply DI2. now apply ZF_refl'.
+Qed.
+
+Lemma opair_inj1 T x y x' y' :
+  ZFeq' <<= T -> T ⊢I opair x y ≡ opair x' y' -> T ⊢I x ≡ x'.
+Proof.
+  intros HT He. assert (H : T ⊢I {x; x} ∈ opair x y).
+  { apply ZF_pair_el'; trivial. apply DI1. now apply ZF_refl'. }
+  eapply ZF_eq_elem in H; try apply He; try apply ZF_refl'; trivial.
+  apply ZF_pair_el' in H; trivial.
+  apply (DE H); eapply sing_pair1; try apply prv_T1; solve_tsub.
+Qed.
+
+Lemma opair_inj2 T x y x' y' :
+  ZFeq' <<= T -> T ⊢I opair x y ≡ opair x' y' -> T ⊢I y ≡ y'.
+Proof.
+  intros HT H. assert (H' : T ⊢I y ≡ x' ∨ y ≡ y').
+  - assert (H2 : T ⊢I {x; y} ∈ opair x' y').
+    { eapply ZF_eq_elem; trivial. apply ZF_refl'; trivial. apply H.
+      apply ZF_pair_el'; trivial. apply DI2. now apply ZF_refl'. }
+    apply ZF_pair_el' in H2; trivial. apply (DE H2).
+    + apply DI1. apply ZF_sym'. solve_tsub. eapply sing_pair2.
+      solve_tsub. apply ZF_sym'; try apply prv_T1. solve_tsub.
+    + apply ZF_pair_el'. solve_tsub. eapply ZF_eq_elem; try apply prv_T1. solve_tsub.
+      apply ZF_refl'. solve_tsub. apply ZF_pair_el'. solve_tsub.
+      apply DI2. apply ZF_refl'. solve_tsub.
+  - apply (DE H'); try apply prv_T1.
+    assert (H1 : T ⊢I x ≡ x') by apply (opair_inj1 HT H).
+    assert (H2 : T ⊢I {x'; y'} ∈ opair x y).
+    { eapply ZF_eq_elem; trivial. apply ZF_refl'; trivial. apply ZF_sym', H; trivial.
+      apply ZF_pair_el'; trivial. apply DI2. now apply ZF_refl'. }
+    apply ZF_pair_el' in H2; trivial.
+    eapply DE; try eapply (Weak_T H2). repeat solve_tsub.
+    + eapply ZF_trans'; try apply prv_T2. repeat solve_tsub.
+      eapply ZF_trans'. repeat solve_tsub. apply ZF_sym'. repeat solve_tsub.
+      apply (Weak_T H1). repeat solve_tsub. eapply sing_pair2. repeat solve_tsub.
+      apply ZF_sym'; try apply prv_T1. repeat solve_tsub.
+    + eapply ZF_trans'; try apply prv_T2. repeat solve_tsub.
+      eapply sing_pair2. repeat solve_tsub. eapply ZF_trans'. repeat solve_tsub.
+      2: apply ZF_sym'; try apply prv_T1. 2: repeat solve_tsub.
+      eapply ZF_eq_pair; try apply ZF_sym'; try apply prv_T2.
+      3: apply (Weak_T H1). all: repeat solve_tsub.
+Qed.
+
+Lemma ZF_bunion_el1 T x y z :
+  ZFeq' <<= T -> T ⊢I z ∈ x -> T ⊢I z ∈ x ∪ y.
+Proof.
+  intros HT H. now apply ZF_bunion_el', DI1.
+Qed.
+
+Lemma ZF_bunion_el2 T x y z :
+  ZFeq' <<= T -> T ⊢I z ∈ y -> T ⊢I z ∈ x ∪ y.
+Proof.
+  intros HT H. now apply ZF_bunion_el', DI2.
+Qed.
+ 
+Lemma bunion_eset x :
+   ZFeq' ⊢I ∅ ∪ x ≡ x.
+Proof.
+  apply ZF_ext'; try apply ZF_all, impl; cbn. solve_tsub. 
+  - eapply DE. eapply ZF_bunion_inv. repeat solve_tsub. apply prv_T1.
+    + apply exf. eapply IE; try apply prv_T1.
+      eapply Weak_T; try apply ZF_eset. repeat solve_tsub.
+    + apply prv_T1.
+  - apply ZF_bunion_el2, prv_T1. repeat solve_tsub.
+Qed.
+
+Lemma bunion_swap x y z :
+  ZFeq' ⊢I (x ∪ y) ∪ z ≡ (x ∪ z) ∪ y.
+Proof.
+  apply ZF_ext'; try apply ZF_all, impl; cbn. solve_tsub.
+  - eapply DE. eapply ZF_bunion_inv. repeat solve_tsub. apply prv_T1.
+    + eapply DE. eapply ZF_bunion_inv. repeat solve_tsub. apply prv_T1.
+      * apply ZF_bunion_el1, ZF_bunion_el1, prv_T1. all: repeat solve_tsub.
+      * apply ZF_bunion_el2, prv_T1. repeat solve_tsub.
+    + apply ZF_bunion_el1, ZF_bunion_el2, prv_T1. all: repeat solve_tsub.
+  - eapply DE. eapply ZF_bunion_inv. repeat solve_tsub. apply prv_T1.
+    + eapply DE. eapply ZF_bunion_inv. repeat solve_tsub. apply prv_T1.
+      * apply ZF_bunion_el1, ZF_bunion_el1, prv_T1. all: repeat solve_tsub.
+      * apply ZF_bunion_el2, prv_T1. repeat solve_tsub.
+    + apply ZF_bunion_el1, ZF_bunion_el2, prv_T1. all: repeat solve_tsub.
+Qed.
+
+Lemma bunion_use T x y z phi :
+  ZFeq' <<= T -> T ⋄ (x ∈ y) ⊢I phi -> T ⋄ (x ≡ z) ⊢I phi -> T ⊢I x ∈ y ∪ sing z --> phi.
+Proof.
+  intros HT H1 H2. apply impl. eapply DE.
+  - eapply ZF_bunion_inv. repeat solve_tsub. apply prv_T1.
+  - apply (Weak_T H1). intros psi. unfold extend, contains. tauto.
+  - eapply remove.
+    + rewrite <- ZF_sing_iff. apply prv_T1. repeat solve_tsub.
+    + apply (Weak_T H2). intros psi. unfold extend, contains. tauto.
+Qed.
+
+Lemma ZF_numeral_trans T n x y :
+  ZFeq' <<= T -> T ⊢I x ∈ tnumeral n --> y ∈ x --> y ∈ tnumeral n.
+Proof.
+  intros HT. induction n; cbn.
+  - apply impl, exf.
+    eapply IE; try apply prv_T1.
+    apply ZF_eset'. repeat solve_tsub.
+  - apply bunion_use; trivial.
+    + apply imp in IHn. apply (imps IHn).
+      apply impl. apply ZF_bunion_el1, prv_T1. repeat solve_tsub.
+    + apply impl. apply ZF_bunion_el'. repeat solve_tsub.
+      apply DI1. eapply ZF_eq_elem; try apply prv_T2; try apply prv_T1.
+      repeat solve_tsub. apply ZF_refl'. repeat solve_tsub.
+Qed.
+
+Lemma ZF_numeral_wf T n :
+  ZFeq' <<= T -> T ⊢I ¬ (tnumeral n ∈ tnumeral n).
+Proof.
+  intros HT. induction n; cbn.
+  - now apply ZF_eset'.
+  - apply bunion_use; trivial.
+    + eapply IE. apply (Weak_T IHn). repeat solve_tsub.
+      eapply IE. eapply IE. apply ZF_numeral_trans. repeat solve_tsub.
+      apply prv_T1. apply ZF_sig_el. repeat solve_tsub.
+    + eapply IE. apply (Weak_T IHn). repeat solve_tsub.
+      eapply ZF_eq_elem. repeat solve_tsub. apply ZF_refl'. repeat solve_tsub.
+      apply prv_T1. apply ZF_sig_el. repeat solve_tsub.
+Qed.
+
+
+
+
+
+(** ** Preservation proof *)
+
+Lemma enc_derivations_base R n :
+  ZFeq' ⊢I {{∅; ∅}; {∅; enc_stack R}} ∈ enc_derivations R n.
+Proof.
+  induction n; cbn.
+  - apply ZF_sing_el.
+  - apply ZF_bunion_el. now apply DI1.
+Qed.
+
+Lemma enc_derivations_step B n :
+  ZFeq' ⊢I opair (tnumeral n) (enc_stack (derivations B n)) ∈ enc_derivations B n.
+Proof.
+  destruct n; cbn.
+  - apply ZF_sing_el.
+  - apply ZF_bunion_el. apply DI2. apply ZF_sing_el.
+Qed.
+
+Lemma enc_stack_spec R s t :
+  s/t el R -> ZFeq' ⊢I opair (enc_string s) (enc_string t) ∈ enc_stack R.
+Proof.
+  induction R as [|[u v] R IH]; cbn; auto.
+  intros [[=]| H]; subst.
+  - apply ZF_bunion_el. apply DI2. apply ZF_sing_el.
+  - apply ZF_bunion_el. apply DI1. now apply IH.
+Qed.
+
+Lemma ZF_derivations_bound T B k n x :
+  ZFeq' <<= T -> T ⊢I opair k x ∈ enc_derivations B n -> T ⊢I k ∈ σ (tnumeral n).
+Proof.
+  induction n in T |- *; cbn; intros HT H.
+  - apply ZF_sing_iff in H; trivial. eapply ZF_eq_elem; trivial.
+    apply ZF_sym'; trivial. eapply opair_inj1; trivial. apply H.
+    apply ZF_refl'; trivial. eapply ZF_bunion_el'; trivial.
+    apply DI2. apply ZF_sing_iff; trivial. apply ZF_refl'; trivial.
+  - apply ZF_bunion_inv in H; trivial. apply (DE H).
+    + apply ZF_bunion_el1. solve_tsub. apply IHn; try apply prv_T1. solve_tsub.
+    + apply ZF_bunion_el2. solve_tsub. apply ZF_sing_iff. solve_tsub.
+      eapply opair_inj1. solve_tsub. apply ZF_sing_iff; try apply prv_T1. solve_tsub.
+Qed.
+
+Lemma enc_derivations_functional B n :
+  ZFeq' ⊢I opair $2 $1 ∈ enc_derivations B n --> opair $2 $0 ∈ enc_derivations B n --> $ 1 ≡ $ 0.
+Proof.
+  induction n; cbn -[derivations].
+  - repeat apply impl. eapply opair_inj2. repeat solve_tsub. eapply ZF_trans'. repeat solve_tsub.
+    + apply ZF_sing_iff; try apply prv_T2. repeat solve_tsub.
+    + apply ZF_sym'. repeat solve_tsub. apply ZF_sing_iff; try apply prv_T1. repeat solve_tsub.
+  - apply bunion_use; try apply bunion_use. 1,2,5: repeat solve_tsub.
+    + repeat apply imp. now apply (Weak_T IHn).
+    + apply exf. eapply IE. apply (@ZF_numeral_wf _ (S n)). solve_tsub.
+      eapply ZF_derivations_bound. solve_tsub. eapply ZF_eq_elem; try apply prv_T2. solve_tsub.
+      2: apply ZF_refl'. 2: solve_tsub. apply ZF_eq_opair. solve_tsub.
+      eapply opair_inj1; try apply prv_T1. solve_tsub. apply ZF_refl'. solve_tsub.
+    + apply exf. eapply IE. apply (@ZF_numeral_wf _ (S n)). solve_tsub.
+      eapply ZF_derivations_bound. solve_tsub. eapply ZF_eq_elem; try apply prv_T1. solve_tsub.
+      2: apply ZF_refl'. 2: solve_tsub. apply ZF_eq_opair. solve_tsub.
+      eapply opair_inj1; try apply prv_T2. solve_tsub. apply ZF_refl'. solve_tsub.
+    + eapply opair_inj2. solve_tsub. eapply ZF_trans'; try apply prv_T2. solve_tsub.
+      apply ZF_sym'; try apply prv_T1. solve_tsub.
+Qed.
+
+Lemma prep_string_subst sigma s x :
+  subst_term sigma (prep_string s x) = prep_string s (subst_term sigma x).
+Proof.
+  induction s; cbn; trivial. rewrite IHs.
+  rewrite substt_bounded0; eauto.
+  apply enc_bool_bounded0.
+Qed.
+
+Lemma is_rep_subst s t x y sigma :
+  subst_form sigma (is_rep (comb_rel s t) x y) =
+  is_rep (comb_rel s t) (subst_term sigma x) (subst_term sigma y).
+Proof.
+  unfold is_rep. cbn -[comb_rel]. asimpl. repeat f_equal.
+  - unfold comb_rel. cbn. rewrite !prep_string_subst. reflexivity.
+  - unfold comb_rel. cbn. rewrite !prep_string_subst. reflexivity.
+Qed.
+
+Lemma combinations_subst B x y sigma :
+  subst_form sigma (combinations B x y) = combinations B (subst_term sigma x) (subst_term sigma y).
+Proof.
+  induction B as [|[s t] B IH] in sigma, x, y |- *.
+  - cbn. reflexivity.
+  - cbn -[is_rep]. rewrite IH, is_rep_subst. cbn -[is_rep]. now asimpl.
+Qed.
+
+Lemma enc_derivations_eq T B n x :
+  ZFeq' <<= T -> T ⊢I opair (tnumeral n) x ∈ enc_derivations B n -> T ⊢I x ≡ enc_stack (derivations B n).
+Proof.
+  intros HT H. destruct n; cbn in *.
+  - eapply opair_inj2; trivial. eapply ZF_sing_iff; eauto.
+  - apply ZF_bunion_inv in H; trivial. apply (DE H).
+    + apply exf. eapply IE. apply (ZF_numeral_wf (S n)). solve_tsub.
+      eapply ZF_derivations_bound. solve_tsub. apply prv_T1.
+    + eapply opair_inj2. solve_tsub. apply ZF_sing_iff. solve_tsub. apply prv_T1.
+Qed.
+
+Lemma enc_stack_app {T} {HB : bounded_theory T} B C :
+  ZFeq' <<= T -> T ⊢I (enc_stack B) ∪ (enc_stack C) ≡ enc_stack (B ++ C).
+Proof.
+  intros HT. induction B as [|[s t] B IH]; cbn.
+  - eapply Weak_T; try apply bunion_eset. assumption.
+  - eapply ZF_trans'; trivial. eapply Weak_T; try apply bunion_swap; trivial.
+    eapply ZF_eq_bunion; trivial. apply ZF_refl'; trivial.
+Qed.
+
+Lemma prep_string_app s t x :
+  prep_string (s ++ t) x = prep_string s (prep_string t x).
+Proof.
+  induction s; cbn; congruence.
+Qed.
+
+Lemma ZF_eq_prep T s x y :
+  ZFeq' <<= T -> T ⊢I x ≡ y -> T ⊢I prep_string s x ≡ prep_string s y.
+Proof.
+  intros HT H. induction s; cbn; try tauto.
+  apply ZF_eq_opair; trivial. now apply ZF_refl'.
+Qed.
+
+Lemma append_all_el T B s t x y :
+  ZFeq' <<= T -> T ⊢I opair x y ∈ enc_stack B
+  -> T ⊢I opair (prep_string s x) (prep_string t y) ∈ enc_stack (append_all B (s/t)).
+Proof.
+  intros HT H. induction B as [|[u v] B IH] in T, HT, H |- *; cbn in *.
+  - apply exf. eapply IE. 2: apply H. now apply ZF_eset'.
+  - eapply (ZF_bunion_el' HT). eapply DE. apply (ZF_bunion_inv HT H).
+    + apply DI1. apply IH; try apply prv_T1. solve_tsub.
+    + assert1 H'. apply ZF_sing_iff in H'; try now solve_tsub.
+      apply DI2. apply ZF_sing_iff. solve_tsub.
+      rewrite !prep_string_app. apply ZF_eq_opair. solve_tsub.
+      * apply ZF_eq_prep. solve_tsub. eapply opair_inj1; eauto. solve_tsub.
+      * apply ZF_eq_prep. solve_tsub. eapply opair_inj2; eauto. solve_tsub.
+Qed.
+
+Lemma is_rep_eq {T} {HB : bounded_theory T} B s t x y :
+  ZFeq' <<= T -> T ⊢I x ≡ enc_stack B -> T ⊢I is_rep (comb_rel s t) x y
+  -> T ⊢I y ≡ enc_stack (append_all B (s / t)).
+Proof.
+  intros HT H1 H2. apply ZF_ext'; trivial.
+  - apply bt_all. intros a. cbn.
+    eapply AllE in H2. cbn -[comb_rel] in H2.
+    eapply CE1 in H2. eapply imps. apply H2.
+    apply impl. assert1 H. use_exists H b. apply prv_clear2. clear H.
+    cbn -[comb_rel]. asimpl. assert1 H. apply CE in H as [H H'].
+    unfold comb_rel at 2 in H'. cbn -[comb_rel] in H'. asimpl in H'.
+    rewrite !prep_string_subst in H'. cbn -[comb_rel] in H'. 
+    use_exists H' c. clear H'.
+    cbn -[comb_rel]. asimpl. rewrite !prep_string_subst. cbn -[comb_rel].
+    assert1 H'. use_exists H' d. clear H'.
+    cbn -[comb_rel]. asimpl. rewrite !prep_string_subst. cbn -[comb_rel]. asimpl.
+    eapply ZF_eq_elem. repeat solve_tsub. apply ZF_sym'. repeat solve_tsub.
+    eapply CE2. apply prv_T1. apply ZF_refl'. repeat solve_tsub.
+    apply append_all_el. repeat solve_tsub.
+    eapply ZF_eq_elem. repeat solve_tsub. eapply CE1. apply prv_T1.
+    eapply (Weak_T H1). repeat solve_tsub. eapply (Weak_T H). repeat solve_tsub.
+  - apply bt_all. intros a. cbn. asimpl.
+    apply (@AllE _ _ _ _ _ a) in H2. cbn -[comb_rel] in H2. asimpl in H2.
+    eapply CE2 in H2. eapply imps. 2: apply H2. clear H2. apply impl.
+    induction B as [|[u v] B IH] in T, x, HT, H1, HB |- *; cbn -[comb_rel] in *.
+    + apply exf. eapply IE; try apply prv_T1. apply ZF_eset'. repeat solve_tsub.
+    + apply imp. apply bunion_use; trivial.
+      * specialize (IH T HB (enc_stack B) HT).
+        assert (H : T ⊢I enc_stack B ≡ enc_stack B) by now apply ZF_refl'.
+        apply IH in H. use_exists H z. clear H. apply ExI with z.
+        cbn -[comb_rel]. asimpl. assert1 H. apply CE in H as [H H'].
+        apply CI; trivial. eapply ZF_eq_elem. repeat solve_tsub.
+        apply ZF_refl'. repeat solve_tsub. apply ZF_sym'. repeat solve_tsub.
+        apply (Weak_T H1). repeat solve_tsub. apply ZF_bunion_el1; trivial. repeat solve_tsub.
+      * apply ExI with (opair (enc_string u) (enc_string v)).
+        cbn -[comb_rel]. asimpl. apply CI.
+        -- eapply ZF_eq_elem. repeat solve_tsub. apply ZF_refl'. repeat solve_tsub.
+           apply ZF_sym'. repeat solve_tsub. apply (Weak_T H1). repeat solve_tsub.
+           apply ZF_bunion_el2. repeat solve_tsub. eapply Weak_T. apply ZF_sing_el.
+           repeat solve_tsub.
+        -- cbn. apply ExI with (enc_string v).
+           cbn. apply ExI with (enc_string u).
+           cbn. asimpl. rewrite !prep_string_subst, !prep_string_app; cbn.
+           apply CI; try apply prv_T1. apply ZF_refl'. repeat solve_tsub.
+Qed.
+
+Lemma combinations_eq {T} {HB : bounded_theory T} B C x y :
+  ZFeq' <<= T -> T ⊢I x ≡ enc_stack C -> T ⊢I combinations B x y -> T ⊢I y ≡ enc_stack (derivation_step B C).
+Proof.
+  induction B as [|[s t] B IH] in y, T, HB |-*; cbn; intros HT H1 H2; trivial.
+  use_exists H2 u. clear H2. cbn -[is_rep]. asimpl. assert1 H. use_exists H v. clear H. apply prv_clear2.
+  cbn -[is_rep]. asimpl. rewrite !combinations_subst, !is_rep_subst. cbn -[is_rep]. asimpl.
+  eapply ZF_trans'. solve_tsub. eapply CE1. apply prv_T1.
+  eapply ZF_trans'. solve_tsub. 2: apply enc_stack_app; eauto. 2: solve_tsub.
+  apply ZF_eq_bunion; eauto. solve_tsub.
+  - eapply is_rep_eq; eauto. solve_tsub. apply prv_clear1. eauto.
+    eapply CE2. eapply CE2. apply prv_T1.
+  - apply IH; eauto. solve_tsub.
+    + now apply prv_clear1.
+    + eapply CE1. eapply CE2. apply prv_T1.
+Qed.
+
+Lemma combinations_step B n (i x y : term) :
+  ZFeq' ⊢I i ∈ tnumeral n --> opair i x ∈ enc_derivations B n
+     --> combinations B x y --> opair (σ i) y ∈ enc_derivations B n.
+Proof.
+  induction n; cbn.
+  - apply impl. apply exf.
+    apply imp. apply ZF_eset.
+  - apply bunion_use; try apply bunion_use.
+    apply tsubs_refl. 1, 4: apply tsubs_extend.
+    + apply impl. apply ZF_bunion_el'. repeat solve_tsub.
+      apply DI1. eapply IE. eapply IE. eapply IE.
+      * eapply Weak_T. apply IHn. repeat solve_tsub.
+      * apply prv_T3.
+      * apply prv_T2.
+      * apply prv_T1.
+    + apply exf. eapply IE. apply (ZF_numeral_wf (S n)). solve_tsub.
+      eapply ZF_eq_elem. solve_tsub. eapply opair_inj1. solve_tsub. apply prv_T1.
+      apply ZF_refl'. solve_tsub. cbn. apply ZF_bunion_el'. solve_tsub.
+      apply DI1. apply prv_T2.
+    + apply impl. apply ZF_bunion_el'. repeat solve_tsub.
+      apply DI2. apply ZF_sing_iff. repeat solve_tsub.
+      apply ZF_eq_opair. repeat solve_tsub.
+      * apply ZF_eq_sig; eauto. repeat solve_tsub. apply prv_T3.
+      * eapply combinations_eq; eauto; try apply prv_T1. repeat solve_tsub.
+        apply enc_derivations_eq. repeat solve_tsub.
+        eapply ZF_eq_elem; try apply prv_T2; try apply ZF_refl'. 1, 3: repeat solve_tsub.
+        eapply ZF_eq_opair; try apply prv_T3; try apply ZF_refl'. all: repeat solve_tsub.
+    + apply exf. eapply IE. apply (ZF_numeral_wf n). solve_tsub.
+      eapply ZF_eq_elem. solve_tsub. apply ZF_refl'. solve_tsub.
+      eapply ZF_trans'. solve_tsub. apply ZF_sym'. solve_tsub.
+      eapply opair_inj1. solve_tsub. apply prv_T1. apply prv_T2.
+      apply ZF_sig_el. solve_tsub.
+Qed.
+
+Theorem BPCP_slv B :
+  BPCP' B -> ZFeq' ⊢I solvable B.
+Proof.
+  intros [s H]. destruct (derivable_derivations H) as [n Hn].
+  apply ExI with (tnumeral n);
+  apply ExI with (enc_derivations B n);
+  apply ExI with (opair (enc_string s) (enc_string s));
+  apply ExI with (enc_string s);
+  apply ExI with (enc_stack (derivations B n)); fold subst_form.
+  cbn; rewrite !substt_bounded0; repeat apply perst_bounded0; eauto.
+  repeat apply CI.
+  - apply ZF_numeral.
+  - repeat apply ZF_all. asimpl. unfold unscoped.shift.
+    apply enc_derivations_functional.
+  - apply enc_derivations_base.
+  - repeat apply ZF_all. rewrite !combinations_subst. cbn. asimpl.
+    rewrite !combinations_subst. cbn. unfold unscoped.shift.
+    apply combinations_step.
+  - apply enc_derivations_step.
+  - now apply enc_stack_spec.
+  - apply ZF_refl.
+Qed.
+
+
+
+
+
+(** ** Main Theorem *)
+
+Theorem dPCP_ZFD B :
+  dPCPb B -> ZFeq' ⊢I solvable B.
+Proof.
+Admitted.
+
 Theorem PCP_ZFD B :
   PCPb B -> ZFeq' ⊢I solvable B.
 Proof.
-Admitted.
+  rewrite PCPb_iff_dPCPb. apply dPCP_ZFD.
+Qed.
+
+
+
 
 
 
